Add export JSON and sample haskell server

haskellServer/src/Lib.hs
@@ -1,0 +1,47 @@
+{-# LANGUAGE DataKinds       #-}
+{-# LANGUAGE TemplateHaskell #-}
+{-# LANGUAGE TypeOperators   #-}
+module Lib
+    ( startApp
+    , app
+    ) where
+
+import Data.Aeson
+import Data.Aeson.TH
+import Network.Wai
+import Network.Wai.Handler.Warp
+import Servant
+import Extracted(exported_get_artist, exported_get_album_and_artist)
+-- Note that after extraction, the extracted file must have the following imports added
+-- import Data.Char
+-- import Data.Bits
+
+-- data User = User
+--   { userId        :: Int
+--   , userFirstName :: String
+--   , userLastName  :: String
+--   } deriving (Eq, Show)
+-- 
+-- $(deriveJSON defaultOptions ''User)
+
+type API = "get_artist_less_than" :> Capture "n" Integer :> Get '[JSON] String
+           :<|> "get_album_and_artist" :> Capture "n" Integer :> Get '[JSON] String
+
+startApp :: IO ()
+startApp = do putStrLn "Starting server on port 8080"
+              run 8080 app
+
+app :: Application
+app = serve api server
+
+api :: Proxy API
+api = Proxy
+
+server :: Server API
+server = get_artist :<|> get_album_and_artist
+  where get_artist :: Integer -> Handler String
+        get_artist x = return $ exported_get_artist x
+
+        get_album_and_artist :: Integer -> Handler String
+        get_album_and_artist x = return $ exported_get_album_and_artist x
+
