haskellServer/test/Spec.hs
@@ -1,0 +1,19 @@
+{-# LANGUAGE QuasiQuotes #-}
+{-# LANGUAGE OverloadedStrings #-}
+module Main (main) where
+
+import Lib (app)
+import Test.Hspec
+import Test.Hspec.Wai
+
+main :: IO ()
+main = hspec spec
+
+spec :: Spec
+spec = with (return app) $ do
+    describe "GET /users" $ do
+        it "responds with 200" $ do
+            get "/users" `shouldRespondWith` 200
+        it "responds with [User]" $ do
+            let users = "[{\"userId\":1,\"userFirstName\":\"Isaac\",\"userLastName\":\"Newton\"},{\"userId\":2,\"userFirstName\":\"Albert\",\"userLastName\":\"Einstein\"}]"
+            get "/users" `shouldRespondWith` users
